James C - cleaning up constraints

isabelle/Chapter13_2_Typechecking.thy
@@ -31,29 +31,6 @@ inductive_cases [elim!]: "typecheck_constr (CInR x y z) t"
 inductive_cases [elim!]: "typecheck_constr CTriv t"
 inductive_cases [elim!]: "typecheck_constr (CPair x y) t"
 
-inductive de_morgan_dual :: "constr => constr => bool"
-where dmdal [simp]: "de_morgan_dual All Nothing"
-    | dmdan [simp]: "de_morgan_dual c1 c1' ==> de_morgan_dual c2 c2' ==> de_morgan_dual (And c1 c2) (Or c1' c2')"
-    | dmdno [simp]: "de_morgan_dual Nothing All"
-    | dmdor [simp]: "de_morgan_dual c1 c1' ==> de_morgan_dual c2 c2' ==> de_morgan_dual (Or c1 c2) (And c1' c2')"
-    | dmdil [simp]: "de_morgan_dual c c' ==> de_morgan_dual (CInL t1 t2 c) (Or (CInL t1 t2 c') (CInR t1 t2 All))"
-    | dmdir [simp]: "de_morgan_dual c c' ==> de_morgan_dual (CInR t1 t2 c) (Or (CInR t1 t2 c') (CInL t1 t2 All))"
-    | dmdtr [simp]: "de_morgan_dual CTriv Nothing"
-    | dmdpr [simp]: "de_morgan_dual c1 c1' ==> de_morgan_dual c2 c2' ==> 
-          de_morgan_dual (CPair c1 c2) (Or (CPair c1' c2) (Or (CPair c1 c2') (CPair c1' c2')))"
-
-inductive_cases [elim!]: "de_morgan_dual All t"
-inductive_cases [elim!]: "de_morgan_dual (And x y) t"
-inductive_cases [elim!]: "de_morgan_dual Nothing t"
-inductive_cases [elim!]: "de_morgan_dual (Or x y) t"
-inductive_cases [elim!]: "de_morgan_dual (CInL x y z) t"
-inductive_cases [elim!]: "de_morgan_dual (CInR x y z) t"
-inductive_cases [elim!]: "de_morgan_dual CTriv t"
-inductive_cases [elim!]: "de_morgan_dual (CPair x y) t"
-
-lemma [simp]: "typecheck_constr c t ==> de_morgan_dual c c' ==> typecheck_constr c' t"
-by (induction c t arbitrary: c' rule: typecheck_constr.induct, auto)
-
 inductive satisfies :: "expr => constr => bool"
 where [simp]: "satisfies e All"
     | [simp]: "satisfies e c1 ==> satisfies e c2 ==> satisfies e (And c1 c2)"
@@ -73,43 +50,38 @@ inductive_cases [elim!]: "satisfies e (CInR x y z)"
 inductive_cases [elim!]: "satisfies e CTriv"
 inductive_cases [elim!]: "satisfies e (CPair x y)"
 
-inductive incon :: "constr list => bool"
-where "incon cs ==> incon (All # cs)"
-    | "incon (c1 # c2 # cs) ==> incon (And c1 c2 # cs)"
-    | "incon (Nothing # cs)"
-    | "incon (c1 # cs) ==> incon (c2 # cs) ==> incon (Or c1 c2 # cs)"
-    | "CInR t1 t2 c' : set cs ==> incon (CInL t1 t2 c # cs)"
-    | "CInL t1 t2 c' : set cs ==> incon (CInR t1 t2 c # cs)"
-    | "ALL c : set cs. EX c'. c = CInL t1 t2 c' ==> incon (map (%c. case c of CInL t t' c' => c') cs) ==> incon cs"
-    | "ALL c : set cs. EX c'. c = CInR t1 t2 c' ==> incon (map (%c. case c of CInR t t' c' => c') cs) ==> incon cs"
-    | "ALL c : set cs. EX c1 c2. c = CPair c1 c2 ==> incon (map (%c. case c of CPair c1 c2 => c1) cs) ==> incon cs"
-    | "ALL c : set cs. EX c1 c2. c = CPair c1 c2 ==> incon (map (%c. case c of CPair c1 c2 => c2) cs) ==> incon cs"
+primrec totally_satisfied :: "type => constr => bool"
+where "totally_satisfied t All = True"
+    | "totally_satisfied t (And c1 c2) = (totally_satisfied t c1 & totally_satisfied t c2)" 
+    | "totally_satisfied t Nothing = False"  
+    | "totally_satisfied t (Or c1 c2) = (totally_satisfied t c1 | totally_satisfied t c2)" 
+    | "totally_satisfied t (CInL t1 t2 c) = (t = Sum t1 t2 & totally_satisfied t1 c)"
+    | "totally_satisfied t (CInR t1 t2 c) = (t = Sum t1 t2 & totally_satisfied t2 c)"
+    | "totally_satisfied t CTriv = (t = Unit)" 
+    | "totally_satisfied t (CPair c1 c2) = (case t of Prod t1 t2 => totally_satisfied t1 c1 & totally_satisfied t2 c2 | _ => False)" 
 
-definition totally_satisfied :: "constr => bool"
-where "totally_satisfied c = incon [THE c'. de_morgan_dual c c']"
+inductive types_from_pat :: "patn => type => type list => bool"
+where tpwld [simp]: "types_from_pat Wild t []"
+    | tpvar [simp]: "types_from_pat PVar t [t]"
+    | tptrv [simp]: "types_from_pat PTriv Unit []"
+    | tppar [simp]: "types_from_pat p1 t1 ts1 ==> types_from_pat p2 t2 ts2 ==> 
+          types_from_pat (PPair p1 p2) (Prod t1 t2) (ts1 @ ts2)"
+    | tpinl [simp]: "types_from_pat p t1 ts ==> types_from_pat (PInL p) (Sum t1 t2) ts"
+    | tpinr [simp]: "types_from_pat p t2 ts ==> types_from_pat (PInR p) (Sum t1 t2) ts"
 
-inductive types_from_pat :: "patn => type => type list => constr => bool"
-where tpwld [simp]: "types_from_pat Wild t [] All"
-    | tpvar [simp]: "types_from_pat PVar t [t] All"
-    | tptrv [simp]: "types_from_pat PTriv Unit [] CTriv"
-    | tppar [simp]: "types_from_pat p1 t1 ts1 c1 ==> types_from_pat p2 t2 ts2 c2 ==> 
-          types_from_pat (PPair p1 p2) (Prod t1 t2) (ts1 @ ts2) (CPair c1 c2)"
-    | tpinl [simp]: "types_from_pat p t1 ts c ==> types_from_pat (PInL p) (Sum t1 t2) ts (CInL t1 t2 c)"
-    | tpinr [simp]: "types_from_pat p t2 ts c ==> types_from_pat (PInR p) (Sum t1 t2) ts (CInR t1 t2 c)"
+inductive_cases [elim!]: "types_from_pat Wild t ts"
+inductive_cases [elim!]: "types_from_pat PVar t ts"
+inductive_cases [elim!]: "types_from_pat PTriv t ts"
+inductive_cases [elim!]: "types_from_pat (PPair p1 p2) t ts"
+inductive_cases [elim!]: "types_from_pat (PInL p) t ts"
+inductive_cases [elim!]: "types_from_pat (PInR p) t ts"
 
-inductive_cases [elim!]: "types_from_pat Wild t ts c"
-inductive_cases [elim!]: "types_from_pat PVar t ts c"
-inductive_cases [elim!]: "types_from_pat PTriv t ts c"
-inductive_cases [elim!]: "types_from_pat (PPair p1 p2) t ts c"
-inductive_cases [elim!]: "types_from_pat (PInL p) t ts c"
-inductive_cases [elim!]: "types_from_pat (PInR p) t ts c"
-
-lemma [simp]: "types_from_pat p t ts c ==> length ts = vars_count p"
-by (induction p t ts c rule: types_from_pat.induct, simp_all)
+lemma [simp]: "types_from_pat p t ts ==> length ts = vars_count p"
+by (induction p t ts rule: types_from_pat.induct, simp_all)
 
 inductive typecheck :: "(nat, type) assoc => expr => type => bool"
-      and typecheck_rules :: "(nat, type) assoc => rule list => type => type => constr => bool"
-      and typecheck_rule :: "(nat, type) assoc => rule => type => type => constr => bool"
+      and typecheck_rules :: "(nat, type) assoc => rule list => type => type => bool"
+      and typecheck_rule :: "(nat, type) assoc => rule => type => type => bool"
 where tvar [simp]: "lookup env v = Some t ==> typecheck env (Var v) t"
     | tzer [simp]: "typecheck env Zero Nat"    
     | tsuc [simp]: "typecheck env n Nat ==> typecheck env (Succ n) Nat"
@@ -127,10 +99,10 @@ where tvar [simp]: "lookup env v = Some t ==> typecheck env (Var v) t"
     | tabt [simp]: "typecheck env e Void ==> typecheck env (Abort t e) t"
     | tinl [simp]: "typecheck env e t1 ==> typecheck env (InL t1 t2 e) (Sum t1 t2)"
     | tinr [simp]: "typecheck env e t2 ==> typecheck env (InR t1 t2 e) (Sum t1 t2)"
-    | tmch [simp]: "typecheck env e t1 ==> typecheck_rules env rs t1 t2 c ==> totally_satisfied c ==> typecheck env (Match e rs) t2" 
-    | tnil [simp]: "typecheck_rules env [] t1 t2 Nothing"
-    | tcns [simp]: "typecheck_rule env r t1 t2 c ==> typecheck_rules env rs t1 t2 cs ==> typecheck_rules env (r # rs) t1 t2 (Or c cs)"
-    | trul [simp]: "types_from_pat p t1 ts c ==> typecheck (extend_env ts env) e t2 ==> typecheck_rule env (Rule p e) t1 t2 c"
+    | tmch [simp]: "typecheck env e t1 ==> typecheck_rules env rs t1 t2 ==> typecheck env (Match e rs) t2" 
+    | tnil [simp]: "typecheck_rules env [] t1 t2"
+    | tcns [simp]: "typecheck_rule env r t1 t2 ==> typecheck_rules env rs t1 t2 ==> typecheck_rules env (r # rs) t1 t2"
+    | trul [simp]: "types_from_pat p t1 ts ==> typecheck (extend_env ts env) e t2 ==> typecheck_rule env (Rule p e) t1 t2"
 
 inductive_cases [elim!]: "typecheck e (Var x) t"
 inductive_cases [elim!]: "typecheck e Zero t"
@@ -147,16 +119,46 @@ inductive_cases [elim!]: "typecheck e (Abort x y) t"
 inductive_cases [elim!]: "typecheck e (InL x y z) t"
 inductive_cases [elim!]: "typecheck e (InR x y z) t"
 inductive_cases [elim!]: "typecheck e (Match x y) t"
-inductive_cases [elim!]: "typecheck_rules e [] t t' c"
-inductive_cases [elim!]: "typecheck_rules e (r # rs) t t' c"
-inductive_cases [elim!]: "typecheck_rule e (Rule x y) t t' c"
-                        
+inductive_cases [elim!]: "typecheck_rules e [] t t'"
+inductive_cases [elim!]: "typecheck_rules e (r # rs) t t'"
+inductive_cases [elim!]: "typecheck_rule e (Rule x y) t t'"
+  
+primrec extract_constraint :: "patn => constr"       
+where "extract_constraint Wild = All"
+    | "extract_constraint PVar = All"
+    | "extract_constraint PTriv = CTriv"
+    | "extract_constraint (PPair p1 p2) = CPair (extract_constraint p1) (extract_constraint p2)"
+    | "extract_constraint (PInL p) = CInL Void Void (extract_constraint p)"
+    | "extract_constraint (PInR p) = CInR Void Void (extract_constraint p)"
+ 
+primrec all_matches_complete :: "expr => bool"
+    and extract_constraints :: "rule list => constr"
+    and extract_constraint_rule :: "rule => constr"
+where "all_matches_complete (Var v) = True" 
+    | "all_matches_complete Zero = True"
+    | "all_matches_complete (Succ e) = all_matches_complete e"
+    | "all_matches_complete (IsZ e1 e2 e3) = (all_matches_complete e1 & all_matches_complete e2 & all_matches_complete e3)"
+    | "all_matches_complete (Lam t e) = all_matches_complete e"
+    | "all_matches_complete (Ap e1 e2) = (all_matches_complete e1 & all_matches_complete e2)"
+    | "all_matches_complete (Fix t e) = all_matches_complete e"
+    | "all_matches_complete Triv = True"
+    | "all_matches_complete (Pair e1 e2) = (all_matches_complete e1 & all_matches_complete e2)"
+    | "all_matches_complete (ProjL e) = all_matches_complete e"
+    | "all_matches_complete (ProjR e) = all_matches_complete e"
+    | "all_matches_complete (Abort t e) = all_matches_complete e"
+    | "all_matches_complete (InL t1 t2 e) = all_matches_complete e"
+    | "all_matches_complete (InR t1 t2 e) = all_matches_complete e"
+    | "all_matches_complete (Match e rs) = (all_matches_complete e & totally_satisfied Void (extract_constraints rs))"
+    | "extract_constraints [] = Nothing"
+    | "extract_constraints (r # rs) = Or (extract_constraint_rule r) (extract_constraints rs)"
+    | "extract_constraint_rule (Rule p e) = (if all_matches_complete e then extract_constraint p else Nothing)"
+
 lemma [simp]: "typecheck env e t ==> typecheck (extend_at env n k) (incr_from n e) t"
-  and [simp]: "typecheck_rules env rs t1 t2 c ==> typecheck_rules (extend_at env n k) (incr_from_rules n rs) t1 t2 c"
-  and [simp]: "typecheck_rule env r t1 t2 c ==> typecheck_rule (extend_at env n k) (incr_from_rule n r) t1 t2 c"
-proof (induction env e t and env rs t1 t2 c and env r t1 t2 c arbitrary: n and n and n rule: typecheck_typecheck_rules_typecheck_rule.inducts)
+  and [simp]: "typecheck_rules env rs t1 t2 ==> typecheck_rules (extend_at env n k) (incr_from_rules n rs) t1 t2"
+  and [simp]: "typecheck_rule env r t1 t2 ==> typecheck_rule (extend_at env n k) (incr_from_rule n r) t1 t2"
+proof (induction env e t and env rs t1 t2 and env r t1 t2 arbitrary: n and n and n rule: typecheck_typecheck_rules_typecheck_rule.inducts)
 case (tvar env v t)
-  thus ?case by (simp add: incr_def) (* TODO: remove incr_def? *)
+  thus ?case by (simp add: incr_def)
 next case tzer
   thus ?case by simp
 next case tsuc
@@ -190,16 +192,15 @@ next case tinl
   thus ?case by simp
 next case tinr
   thus ?case by simp
-next case (tmch env e t1 rs t2 c)
+next case (tmch env e t1 rs t2)
   hence "typecheck (extend_at env n k) (incr_from n e) t1" by simp
-  moreover from tmch have "typecheck_rules (extend_at env n k) (incr_from_rules n rs) t1 t2 c" by simp
-  moreover from tmch have "totally_satisfied c" by simp
+  moreover from tmch have "typecheck_rules (extend_at env n k) (incr_from_rules n rs) t1 t2" by simp
   ultimately show ?case by simp
 next case tnil
   thus ?case by simp
 next case tcns
   thus ?case by simp
-next case (trul p t1 ts c env e t2)
+next case (trul p t1 ts env e t2)
   from trul have "vars_count p = length ts" by simp
   moreover from trul have "typecheck (extend_at (extend_env ts env) (n + vars_count p) k) (incr_from (n + vars_count p) e) t2" by simp
   ultimately have "typecheck (extend_env ts (extend_at env n k)) (incr_from (n + vars_count p) e) t2" by simp
@@ -210,9 +211,9 @@ lemma [simp]: "typecheck env e t ==> typecheck (extend_env ts env) (incr_by (len
 by (induction ts, simp_all)        
 
 lemma [simp]: "typecheck (extend_at env n k) e t ==> n ~: free_vars e ==> typecheck env (sub_from n e) t"
-  and [simp]: "typecheck_rules (extend_at env n k) rs t1 t2 c ==> n ~: free_vars_rules rs ==> typecheck_rules env (sub_from_rules n rs) t1 t2 c"
-  and [simp]: "typecheck_rule (extend_at env n k) r t1 t2 c ==> n ~: free_vars_rule r ==> typecheck_rule env (sub_from_rule n r) t1 t2 c"
-proof (induction "extend_at env n k" e t and "extend_at env n k" rs t1 t2 c and "extend_at env n k" r t1 t2 c
+  and [simp]: "typecheck_rules (extend_at env n k) rs t1 t2 ==> n ~: free_vars_rules rs ==> typecheck_rules env (sub_from_rules n rs) t1 t2"
+  and [simp]: "typecheck_rule (extend_at env n k) r t1 t2 ==> n ~: free_vars_rule r ==> typecheck_rule env (sub_from_rule n r) t1 t2"
+proof (induction "extend_at env n k" e t and "extend_at env n k" rs t1 t2 and "extend_at env n k" r t1 t2
        arbitrary: env n and env n and env n rule: typecheck_typecheck_rules_typecheck_rule.inducts)
 case (tvar v t)
   thus ?case by (cases "v < n", simp, cases "v = n", simp_all)
@@ -248,10 +249,9 @@ next case tinl
   thus ?case by simp
 next case tinr
   thus ?case by simp
-next case (tmch e t1 rs t2 c)
-  hence "typecheck_rules env (sub_from_rules n rs) t1 t2 c" by simp 
+next case (tmch e t1 rs t2)
+  hence "typecheck_rules env (sub_from_rules n rs) t1 t2" by simp 
   moreover from tmch have "typecheck env (sub_from n e) t1" by simp
-  moreover from tmch have "totally_satisfied c" by simp
   ultimately show ?case by simp
 next case tnil
   thus ?case by simp
@@ -263,9 +263,9 @@ next case (trul p t1 ts)
 qed
 
 lemma [simp]: "typecheck (extend env x t2) e t1 ==> typecheck env eb t2 ==> typecheck env (subst e eb x) t1"
-  and [simp]: "typecheck_rules (extend env x t2) rs t1a t1b c ==> typecheck env eb t2 ==> typecheck_rules env (subst_rules rs eb x) t1a t1b c"
-  and [simp]: "typecheck_rule (extend env x t2) r t1a t1b c ==> typecheck env eb t2 ==> typecheck_rule env (subst_rule r eb x) t1a t1b c"
-proof (induction "extend env x t2" e t1 and "extend env x t2" rs t1a t1b c and "extend env x t2" r t1a t1b c
+  and [simp]: "typecheck_rules (extend env x t2) rs t1a t1b ==> typecheck env eb t2 ==> typecheck_rules env (subst_rules rs eb x) t1a t1b"
+  and [simp]: "typecheck_rule (extend env x t2) r t1a t1b ==> typecheck env eb t2 ==> typecheck_rule env (subst_rule r eb x) t1a t1b"
+proof (induction "extend env x t2" e t1 and "extend env x t2" rs t1a t1b and "extend env x t2" r t1a t1b
        arbitrary: env eb x and env eb x and env eb x rule: typecheck_typecheck_rules_typecheck_rule.inducts)
 case tvar
   thus ?case by auto
@@ -299,10 +299,9 @@ next case tinl
   thus ?case by simp
 next case tinr
   thus ?case by simp
-next case (tmch e t1 rs t2 c)
+next case (tmch e t1 rs t2)
   hence "typecheck env (subst e eb x) t1" by simp
-  moreover from tmch have "typecheck_rules env (subst_rules rs eb x) t1 t2 c" by simp
-  moreover from tmch have "totally_satisfied c" by simp
+  moreover from tmch have "typecheck_rules env (subst_rules rs eb x) t1 t2" by simp
   ultimately show ?case by simp
 next case tnil
   thus ?case by simp
